[minor] Start conversion of RefinementQAC.v.

pico-ifc-coq/dyn_allocation/CLattices.v
@@ -74,10 +74,17 @@ Proof.
   econstructor; econstructor; apply EXT; eauto.
 Qed.
 
+Definition kernel_memory_update (m m' : memory) : Prop :=
+  forall b fr,
+    Mem.stamp b = Kernel ->
+    b <> cblock ->
+    Mem.get_frame m b = Some fr ->
+    Mem.get_frame m' b = Some fr.
+
 Inductive mem_eq_except_cache (m m' : memory) : Prop :=
 | meec_intro :
     mem_def_on_cache m ->
-    fault_handler_memory_update cblock m m' ->
+    kernel_memory_update m m' ->
     mem_eq_except_cache m m'.
 
 Class WfConcreteLattice (T: Type) (L : JoinSemiLattice T) (CL: ConcreteLattice T) :=
